commutativity2.thy
@@ -1,0 +1,17 @@
+theory commutativity2
+imports commutativity
+begin
+
+lemma move_outside_transaction:
+  assumes b_is_a_different_session[simp]: "sa \<noteq> sb"
+    and wf[simp]: "state_wellFormed S"
+    and no_end_atomic: "b \<noteq> AEndAtomic"
+  shows "(S ~~ [(sa,ABeginAtomic t newTxns),(sb,b)] \<leadsto>* T)
+   \<longleftrightarrow> (S ~~ [(sb,b),(sa,ABeginAtomic t newTxns)] \<leadsto>* T)"
+proof (rule useCommutativeS)
+  show "commutativeS S (sa, ABeginAtomic t newTxns) (sb, b)"
+    using assms by (rule commutative_beginAtomic_other)
+qed
+
+
+end
