consistency.thy
@@ -1,0 +1,99 @@
+theory consistency
+imports repliss_sem execution_invariants
+begin
+
+
+
+definition
+"causallyConsistent hb vis \<equiv>
+  (\<forall>c1 c2. c1\<in>vis \<and> (c2,c1)\<in> hb \<longrightarrow> c2\<in>vis)"
+
+definition
+"transactionConsistent origin txStatus vis \<equiv>
+    (\<forall>c tx. c\<in>vis \<and> origin c \<triangleq> tx \<longrightarrow> txStatus tx \<triangleq> Committed)
+  \<and> (\<forall>c1 c2. c1\<in>vis \<and> origin c1 = origin c2 \<longrightarrow> c2\<in>vis)"
+
+lemma transactionConsistent_Committed:
+shows "\<lbrakk>transactionConsistent origin txStatus vis; c\<in>vis; origin c \<triangleq> tx; origin c \<triangleq> tx\<rbrakk> \<Longrightarrow> txStatus tx \<triangleq> Committed"
+by (auto simp add:  transactionConsistent_def) 
+
+lemma transactionConsistent_all_from_same:
+shows "\<lbrakk>transactionConsistent origin txStatus vis; c1\<in>vis; origin c1 = origin c2\<rbrakk> \<Longrightarrow> c2\<in>vis"
+by (auto simp add:  transactionConsistent_def) 
+
+definition consistentSnapshotH where
+"consistentSnapshotH s_calls s_happensBefore s_callOrigin s_transactionStatus vis \<equiv>
+  vis \<subseteq> dom s_calls
+ \<comment> \<open>  causally consistent  \<close> 
+ \<and> (causallyConsistent s_happensBefore vis)
+ \<comment> \<open> transaction consistent  \<close>
+ \<and> (transactionConsistent s_callOrigin s_transactionStatus vis)
+"
+
+abbreviation consistentSnapshot where
+"consistentSnapshot state vis \<equiv>
+consistentSnapshotH (calls state) (happensBefore state) (callOrigin state) (transactionStatus state) vis"
+
+abbreviation consistentSnapshotI where
+"consistentSnapshotI state vis \<equiv>
+consistentSnapshotH (calls state) (happensBefore state) (callOrigin state) (\<lambda>t. Some Committed) vis"
+
+
+lemma show_consistentSnapshot:
+  assumes "vis \<subseteq> dom s_calls"
+and "causallyConsistent s_happensBefore vis"
+and "transactionConsistent s_callOrigin s_transactionStatus vis"
+  shows "consistentSnapshotH s_calls s_happensBefore s_callOrigin s_transactionStatus vis"
+  using assms by (auto simp add: consistentSnapshotH_def)
+
+
+
+lemma chooseSnapshot_causallyConsistent_preserve:
+  assumes a1: "chooseSnapshot snapshot vis S"
+    and a2': "trans (happensBefore S)"
+    and a3: "causallyConsistent (happensBefore S) vis"
+  shows "causallyConsistent (happensBefore S) snapshot"
+  using a1 a3 apply (auto simp add: chooseSnapshot_def downwardsClosure_def causallyConsistent_def)
+   apply (rule_tac x=y in exI)
+  apply auto
+  by (meson a2' transE)
+
+
+
+lemma wellFormed_state_causality:
+assumes wf: "state_wellFormed S"
+shows "\<And>s vis. visibleCalls S s \<triangleq> vis \<longrightarrow> causallyConsistent (happensBefore S) vis"
+  and "trans (happensBefore S)"
+using assms  proof (induct rule: wellFormed_induct)
+  case initial
+  show "visibleCalls (initialState (prog S)) s \<triangleq> vis \<longrightarrow> causallyConsistent (happensBefore (initialState (prog S))) vis" for s vis
+    by (auto simp add: initialState_def)
+  show "trans (happensBefore (initialState (prog S)))"
+    by (auto simp add: initialState_def)
+next
+  case (step C a C')
+
+  have causal: "causallyConsistent (happensBefore C) vis" if "visibleCalls C s \<triangleq> vis" for s vis
+    using step.hyps(2) that by auto
+    
+  
+    
+  show "trans (happensBefore C')"
+    using \<open>trans (happensBefore C)\<close> \<open>C ~~ a \<leadsto> C'\<close> apply (auto simp add: step_simps_all)
+    using causal apply (auto simp add: causallyConsistent_def)
+    by (smt Un_iff domIff empty_iff insert_iff mem_Sigma_iff step.hyps(1) subset_eq trans_def wellFormed_visibleCallsSubsetCalls_h(1))
+    
+  show "visibleCalls C' s \<triangleq> vis \<longrightarrow> causallyConsistent (happensBefore C') vis" for s vis
+    using causal \<open>C ~~ a \<leadsto> C'\<close> apply (auto simp add: step_simps_all)
+        apply (auto simp add: causallyConsistent_def split: if_splits)
+    apply (meson causallyConsistent_def chooseSnapshot_causallyConsistent_preserve step.hyps(3))
+    apply (metis (no_types, lifting) SigmaD2 domIff step.hyps(1) subsetCE wellFormed_visibleCallsSubsetCalls_h(1))
+    using step.hyps(1) wellFormed_visibleCallsSubsetCalls2 by blast
+    
+qed
+
+
+
+end
+
+
