examples.thy
@@ -1,0 +1,41 @@
+theory examples
+imports commutativity
+begin
+
+section "Examples"
+
+text "Various examples to illustrate definitions."
+
+\<comment> \<open>counts how many concurrent transactions are active\<close>
+definition transactionsArePackedMeasure :: "'any trace \<Rightarrow> nat" where
+  "transactionsArePackedMeasure tr \<equiv>
+\<Sum>i\<in>{..<length tr}. card (sessionsInTransaction tr i - {fst (tr!i)})  "
+
+
+theorem not_packed_example2:
+  assumes notPacked: "transactionsArePackedMeasure tr > 0"
+  shows "\<exists>i s a.
+    i<length tr
+  \<and> tr!i = (s,a)
+  \<and> sessionsInTransaction tr i - {s} \<noteq> {}" (is ?goal)
+proof -
+  from notPacked
+  have "0 < (\<Sum>i<length tr. card (sessionsInTransaction tr i - {fst (tr ! i)}))"
+    by (auto simp add: transactionsArePackedMeasure_def)
+  from this 
+  obtain i 
+    where a: "i < length tr" 
+      and b: "card (sessionsInTransaction tr i - {fst (tr ! i)}) > 0"
+    by (meson lessThan_iff not_less sum_nonpos)
+
+  from b 
+  have "sessionsInTransaction tr i - {fst (tr!i)} \<noteq> {}"
+    by fastforce
+
+  then show ?thesis
+    by (metis a prod.collapse)
+qed  
+
+
+
+end
