execution_invariants2.thy
@@ -1,0 +1,13 @@
+theory execution_invariants2
+  imports repliss_sem execution_invariants consistency commutativity
+begin
+
+
+lemma wf_transaction_status_iff_origin_dom:
+  assumes wf: "state_wellFormed S"
+  shows "dom (transactionOrigin S) = dom (transactionStatus S)"
+  by (smt Collect_cong dom_def local.wf wf_transaction_status_iff_origin)
+
+
+
+end
