execution_invariants_unused.thy
@@ -1,0 +1,192 @@
+theory execution_invariants_unused
+  imports repliss_sem execution_invariants consistency commutativity
+begin
+
+text "These are currently unused execution invariants"
+
+
+
+
+lemma causallyConsistent_downwards_closure:
+assumes wf: "state_wellFormed S"
+shows "causallyConsistent (happensBefore S) (cs \<down> happensBefore S)"
+apply (auto simp add: causallyConsistent_def downwardsClosure_def)
+  by (meson local.wf transD wellFormed_state_causality(2))
+
+
+
+lemma consistentSnapshot_txns:
+assumes wf: "state_wellFormed S"
+  and comitted: "txns \<subseteq> committedTransactions S"
+shows "consistentSnapshot S (callsInTransaction S txns \<down> happensBefore S)"
+unfolding consistentSnapshotH_def proof (intro conjI)
+ 
+  show "callsInTransaction S txns \<down> happensBefore S \<subseteq> dom (calls S)"
+    apply (auto simp add: callsInTransactionH_def downwardsClosure_def)
+    using local.wf wellFormed_callOrigin_dom2 apply fastforce
+    by (simp add: domD happensBefore_in_calls_left local.wf)
+    
+  show "causallyConsistent (happensBefore S) (callsInTransaction S txns \<down> happensBefore S)"
+    apply (auto simp add: callsInTransactionH_def downwardsClosure_def causallyConsistent_def)
+    by (meson happensBefore_transitive local.wf transD)
+    
+  show "transactionConsistent (callOrigin S) (transactionStatus S) (callsInTransaction S txns \<down> happensBefore S)"
+  proof (induct rule: show_transactionConsistent)
+    case (only_committed c tx)
+    then show ?case 
+      apply (auto simp add: callsInTransactionH_def downwardsClosure_def)
+      using comitted apply blast
+      using comitted local.wf wellFormed_state_transaction_consistent(4) by fastforce
+  next
+    case (all_from_same c1 c2)
+    then show ?case 
+      apply (auto simp add: callsInTransactionH_def downwardsClosure_def)
+      by (metis local.wf wellFormed_state_transaction_consistent(3))
+  qed
+qed    
+
+
+
+
+
+lemma wellFormed_visibleCallsSubsetCalls:
+  assumes a1: "state_wellFormed A"
+    and a2: "visibleCalls A s \<triangleq> vis"
+  shows "vis \<subseteq> dom (calls A)"
+  using a1 a2 wellFormed_visibleCallsSubsetCalls_h(2) by blast
+
+
+
+lemma wf_current_tx_not_before_others: 
+  assumes wf: "state_wellFormed S"
+    and "visibleCalls S i \<triangleq> Vis"
+    and "currentTransaction S i \<triangleq> tx"
+    and "callOrigin S x \<triangleq> tx"
+    and "callOrigin S y \<noteq> Some tx"
+  shows "(x,y) \<notin> happensBefore S"
+proof -
+  obtain tt :: "(callId \<Rightarrow> txid option) \<Rightarrow> callId \<Rightarrow> txid" where
+    "\<forall>x0 x1. (\<exists>v2. x0 x1 \<triangleq> v2) = x0 x1 \<triangleq> tt x0 x1"
+    by moura
+  then have "\<forall>c f. c \<notin> dom f \<or> f c \<triangleq> tt f c"
+    by blast
+  then have "(x, y) \<notin> happensBefore S \<or> y \<notin> dom (callOrigin S)"
+    by (metis (no_types) assms(3) assms(4) assms(5) local.wf option.inject transactionStatus.distinct(1) wellFormed_currentTransaction_unique_h(2) wellFormed_state_transaction_consistent(4))
+  then show ?thesis
+    by (meson domIff local.wf wellFormed_callOrigin_dom3 wellFormed_happensBefore_calls_r)
+qed
+
+
+(*
+lemma wf_happensBefore_trans: 
+  assumes  wf: "state_wellFormed S"
+  shows "trans (happensBefore S)"
+  using assms apply (induct rule: wellFormed_induct)
+   apply (simp add: initialState_def)
+  apply (auto simp add: step.simps)
+  apply (subst trans_def)
+  apply (auto dest: transD)
+proof -
+
+show "(x, c) \<in> happensBefore t"
+    if c0: "state_wellFormed t"
+   and c1: "trans (happensBefore t)"
+   and c2: "localState t sa \<triangleq> ls"
+   and c3: "currentProc t sa \<triangleq> f"
+   and c4: "f ls = DbOperation Op args ls'"
+   and c5: "currentTransaction t sa \<triangleq> ta"
+   and c6: "calls t c = None"
+   and c7: "querySpec (prog t) Op args (getContextH (calls t) (happensBefore t) (Some vis)) res"
+   and c8: "visibleCalls t sa \<triangleq> vis"
+   and c9: "(x, y) \<in> happensBefore t"
+   and c10: "y \<in> vis"
+   and c11: "x \<notin> vis"
+   for  t sa ls f Op args ls' ta c res vis x y
+  using wellFormed_visibleCallsSubsetCalls[OF c0 c8] wellFormed_visibleCallsSubsetCalls_h(1)[OF c0]
+that 
+*)
+
+
+lemma downwardsClosure_subset2:
+  "x \<in> S \<down> R \<Longrightarrow> x \<in> S \<union> fst ` R"
+  by (meson downwardsClosure_subset subsetCE)
+
+
+text \<open>
+ There can be no action on a invocId after a fail or return:
+ (except for invariant checks)
+\<close>
+lemma nothing_after_fail_or_return:
+  assumes steps: "initialState program ~~ tr \<leadsto>* S"
+    and fail_or_return: "tr!i = (s, AFail) \<or> tr!i = (s, AReturn res)"
+    and i_in_range: "i < length tr"
+  shows "\<nexists>j. j>i \<and> j<length tr \<and> fst(tr!j) = s \<and> \<not>is_AInvcheck (snd (tr!j))" 
+  using steps fail_or_return i_in_range proof (induct rule: steps_induct)
+  case initial
+  then show ?case by auto
+next
+  case (step S' tr a S'')
+  show "\<not> (\<exists>j>i. j < length (tr @ [a]) \<and> fst ((tr @ [a]) ! j) = s \<and> \<not> is_AInvcheck (snd ((tr @ [a]) ! j)))"
+  proof (rule ccontr, auto)
+    fix j
+    assume a1: "j < Suc (length tr)"
+      and a2: "i < j"
+      and a3: "s = fst ((tr @ [a]) ! j)"
+      and a4: "\<not> is_AInvcheck (snd ((tr @ [a]) ! j))"
+
+    have j_def: "j = length tr"
+    proof (rule ccontr)
+      assume "j \<noteq> length tr"
+      then have "j < length tr" using a1 by simp
+      then have "s \<noteq> fst ((tr @ [a]) ! j)"
+        by (metis a2 a4 length_append_singleton less_Suc_eq nth_append order.asym step.IH step.prems(1) step.prems(2))
+      with a3 show False by simp
+    qed
+
+    obtain a_op where a_def: "a = (s, a_op)" using j_def a3
+      by (metis nth_append_length prod.collapse) 
+
+
+
+    from \<open>(tr @ [a]) ! i = (s, AFail) \<or> (tr @ [a]) ! i = (s, AReturn res)\<close>
+    have no_ls: "localState S' s = None" 
+      and op: "invocationOp S' s \<noteq> None"  
+       apply (metis a2 everything_starts_with_an_invocation j_def nth_append step.steps)
+      by (metis a2 everything_starts_with_an_invocation j_def nth_append step.prems(1) step.steps)
+
+    have fst_a: "fst a = s" using a_def by simp  
+
+    from \<open>S' ~~ a \<leadsto> S''\<close> a_def
+    have "S' ~~ (s, a_op) \<leadsto> S''" by simp  
+
+    then show False
+      apply (rule step.cases)
+              apply (auto simp add: no_ls a3 op j_def)
+              apply (auto simp add: fst_a no_ls op)
+      using a4 a_def is_AInvcheck_def j_def by auto 
+  qed
+qed
+
+
+
+text \<open>
+ We have visible calls iff we have some local state.
+\<close>
+lemma visibleCalls_iff_localState:
+  assumes steps: "initialState program ~~ tr \<leadsto>* S"
+  shows "localState S s = None \<longleftrightarrow> visibleCalls S s = None" 
+  using steps
+proof (induct rule: steps_induct)
+  case initial
+  then show ?case
+    by (simp add: initialState_def)
+next
+  case (step S' tr a S'')
+  from \<open>S' ~~ a \<leadsto> S''\<close>
+  show ?case 
+    apply (rule step.cases)
+    using step.IH  by (auto simp add: step)
+qed
+
+
+end
